chore: show how we lose defeqs if we use hashmap. This is not clear to me why

Tactics/ArmConstr.lean
@@ -15,6 +15,31 @@ inspired by `simp_arith`, especially the following files:
 
 import Arm.Exec
 
+
+namespace Std.HashMap
+
+def extEq [BEq α] [Hashable α] [Inhabited β] (m1 m2 : Std.HashMap α β) : Prop :=
+  m1.size = m2.size ∧  ∀ (k : α), Std.HashMap.get? m1 k = Std.HashMap.get? m2 k
+
+-- #check BitVec.instDecidableForallBitVec
+
+def extEqb [BEq α] [Hashable α] [Inhabited β] [DecidableEq β] (m1 m2 : Std.HashMap α β) : Bool :=
+  m1.size = m2.size &&
+  m1.fold (init := true) (fun b k v => b && (match Std.HashMap.get? m2 k with
+                                              | some v' => v == v'
+                                              | none => false))
+
+theorem extEq_iff_extEqb : ∀ [BEq α] [Hashable α] [Inhabited β] [DecidableEq β]
+  (m1 m2 : Std.HashMap α β), extEq m1 m2 ↔ extEqb m1 m2 := sorry
+
+instance [BEq α] [Hashable α] (m1 m2 : Std.HashMap α β) [Inhabited β] [DecidableEq β] :
+    Decidable (extEq m1 m2) := by
+  rw [extEq_iff_extEqb]
+  infer_instance
+
+end Std.HashMap
+
+
 namespace ArmConstr
 
 /- We use `Nat`s to refer to all the state variables in our context. -/
@@ -32,8 +57,8 @@ inductive GPRVal where
   | r_gpr (i : BitVec 5)
   deriving DecidableEq, Repr, Inhabited
 
-abbrev StateContext := List ArmState
-abbrev GPRValContext := List (BitVec 64)
+abbrev StateVarContext := List ArmState
+abbrev GPRVarContext := Std.HashMap Nat <| BitVec 64
 
 /--
 Context containing all the variables encountered in the problem. The
@@ -41,58 +66,57 @@ position of a variable in the context becomes variable name (see, e.g.,
 `StateVar`, which is a `Nat`).
 -/
 structure Context where
-  Γs : StateContext
-  Γgpr : GPRValContext
+  Γs : StateVarContext
+  Γgpr : GPRVarContext
   deriving Repr, Inhabited
-
 /--
-Look up variable `v` in the `StateContext`.
+Look up variable `v` in the `StateVarContext`.
 -/
-def StateVar.denote (ctx : StateContext) (v : StateVar) : ArmState :=
+def StateVar.denote (ctx : StateVarContext) (v : StateVar) : ArmState :=
   ctx.getD v ArmState.default
 
 /--
 Denote `GPRVal v`.
 
-If `v` is a variable then look it up in the `GPRValContext`. Else if `v` is
+If `v` is a variable then look it up in the `GPRVarContext`. Else if `v` is
 `r_gpr i`, then look up the `i`th register in `prev_s`.
 -/
-def GPRVal.denote (ctx : GPRValContext) (v : GPRVal) (prev_s : ArmState) : BitVec 64 :=
+def GPRVal.denote (ctx : GPRVarContext) (v : GPRVal) (prev_s : ArmState) : BitVec 64 :=
   match v with
-  | var i => ctx.getD i 0
+  | var i => ctx.getD i 0#64
   | r_gpr i => r (.GPR i) prev_s
 
-/--
-Datastructure that characterizes all the updates that can be made to an
-`ArmState`.
--/
-inductive Update where
-  -- `i` is a constant.
-  | w_gpr (i : BitVec 5) (v : GPRVal)
-  -- TODO: Other state components.
-  deriving DecidableEq, Repr, Inhabited
+-- /--
+-- Datastructure that characterizes all the updates that can be made to an
+-- `ArmState`.
+-- -/
+-- inductive Update where
+--   -- `i` is a constant.
+--   | w_gpr (i : BitVec 5) (v : GPRVal)
+--   -- TODO: Other state components.
+--   deriving DecidableEq, Repr, Inhabited
 
-/--
-Do updates `x` and `y` refer to the same state component?
--/
-def Update.regEq (x y : Update) : Prop :=
-  match x, y with
-  | w_gpr i _, w_gpr j _ => i = j
+-- /--
+-- Do updates `x` and `y` refer to the same state component?
+-- -/
+-- def Update.regEq (x y : Update) : Prop :=
+--   match x, y with
+--   | w_gpr i _, w_gpr j _ => i = j
 
-instance : Decidable (Update.regEq x y) := by
-  simp [Update.regEq]
-  infer_instance
+-- instance : Decidable (Update.regEq x y) := by
+--   simp [Update.regEq]
+--   infer_instance
 
-/--
-Is the register index of update `x` less than that of `y`?
--/
-def Update.regIndexLt (x y : Update) : Prop :=
-  match x, y with
-  | w_gpr i _, w_gpr j _ => i < j
+-- /--
+-- Is the register index of update `x` less than that of `y`?
+-- -/
+-- def Update.regIndexLt (x y : Update) : Prop :=
+--   match x, y with
+--   | w_gpr i _, w_gpr j _ => i < j
 
-instance : Decidable (Update.regIndexLt x y) := by
-  simp [Update.regIndexLt]
-  infer_instance
+-- instance : Decidable (Update.regIndexLt x y) := by
+--   simp [Update.regIndexLt]
+--   infer_instance
 
 /--
 Datastructure to represent expressions characterizing the following state
@@ -105,27 +129,39 @@ curr_state = writes[prev_state]
 structure Expr where
    curr_state : StateVar
    prev_state : StateVar
-   writes : List Update -- Sorted by the state components.
-deriving DecidableEq, Repr, Inhabited
+   writes : Std.HashMap (BitVec 5) GPRVal -- Sorted by the state components.
+deriving Repr, Inhabited
 
-/--
-Map updates `us` to state `prev_state` to an `ArmState`.
--/
-def Expr.writes.denote (ctx : Context) (us : List Update) (prev_state : StateVar)
-  : ArmState :=
-  match us with
-  | [] => StateVar.denote ctx.Γs prev_state
-  | Update.w_gpr i v :: rest =>
-    w (.GPR i)
-      (GPRVal.denote ctx.Γgpr v (StateVar.denote ctx.Γs prev_state))
-      (Expr.writes.denote ctx rest prev_state)
+def Expr.denote_writes (ctx : Context) (e : Expr) (s0 : StateVar) : ArmState :=
+  let s1 := StateVar.denote ctx.Γs s0
+  e.writes.fold (init := s1) (fun s i v => w (.GPR i) (GPRVal.denote ctx.Γgpr v s) s)
+
+def Expr.denote_eq? (e1 e2 : Expr) : Prop :=
+  e1.curr_state = e2.curr_state ∧
+  e1.prev_state = e2.prev_state ∧
+  e1.writes.extEq e2.writes
+
+instance : Decidable (Expr.denote_eq? e1 e2) := by
+  simp [Expr.denote_eq?]
+  infer_instance
+
+-- /--
+-- Map updates `us` to state `prev_state` to an `ArmState`.
+-- -/
+-- def Expr.writes.denote (ctx : Context) (us : List Update) (prev_state : StateVar)
+--   : ArmState :=
+--   match us with
+--   | [] => StateVar.denote ctx.Γs prev_state
+--   | Update.w_gpr i v :: rest =>
+--     w (.GPR i)
+--       (GPRVal.denote ctx.Γgpr v (StateVar.denote ctx.Γs prev_state))
+--       (Expr.writes.denote ctx rest prev_state)
 
 /--
 Denote an `Expr e` to a `Prop` corresponding to `curr_state = writes[prev_state]`.
 -/
 def Expr.denote (ctx : Context) (e : Expr) : Prop :=
-  StateVar.denote ctx.Γs e.curr_state =
-  Expr.writes.denote ctx e.writes e.prev_state
+  StateVar.denote ctx.Γs e.curr_state = Expr.denote_writes ctx e e.prev_state
 
 /--
 Return a `Prop` corresponding to `e1 = e2`.
@@ -145,100 +181,101 @@ def Exprs.denote (ctx : Context) (es : Exprs) : Prop :=
   es.foldl (init := True) (fun p e => p ∧ e.denote ctx)
 
 def Expr.default : Expr :=
-  { prev_state := 0, curr_state := 0, writes := [] }
+  { prev_state := 0, curr_state := 0, writes := ∅ }
 
-def Update.insertSorted (es : List Update) (u : Update) : List Update :=
-  match es with
-  | [] => [u]
-  | e :: rest =>
-    if u.regIndexLt e then
-      -- `u` does not appear in `es` (given that `es` is sorted), so we retain
-      -- this update.
-      u :: es
-    else if u.regEq e then
-      -- We overwrite `e` with `x`.
-      u :: rest
-    else
-      e :: (insertSorted rest u)
+-- def Update.insertSorted (es : List Update) (u : Update) : List Update :=
+--   match es with
+--   | [] => [u]
+--   | e :: rest =>
+--     if u.regIndexLt e then
+--       -- `u` does not appear in `es` (given that `es` is sorted), so we retain
+--       -- this update.
+--       u :: es
+--     else if u.regEq e then
+--       -- We overwrite `e` with `x`.
+--       u :: rest
+--     else
+--       e :: (insertSorted rest u)
 
-/--
-Resolve any reads in `u` by looking it up in `es`.
--/
-def Update.resolveRead (es : List Update) (u : Update) : Update :=
-  match u with
-  | .w_gpr _ (.var _) => u
-  | .w_gpr i (.r_gpr gpr_idx) =>
-    let ans := go gpr_idx es
-    .w_gpr i ans
-  where go (gpr_idx : BitVec 5) (es : List Update) : GPRVal :=
-    match es with
-    | [] => .r_gpr gpr_idx
-    | (.w_gpr i v) :: rest =>
-      if i == gpr_idx then v else go gpr_idx rest
+-- /--
+-- Resolve any reads in `u` by looking it up in `es`.
+-- -/
+-- def Update.resolveRead (es : List Update) (u : Update) : Update :=
+--   match u with
+--   | .w_gpr _ (.var _) => u
+--   | .w_gpr i (.r_gpr gpr_idx) =>
+--     let ans := go gpr_idx es
+--     .w_gpr i ans
+--   where go (gpr_idx : BitVec 5) (es : List Update) : GPRVal :=
+--     match es with
+--     | [] => .r_gpr gpr_idx
+--     | (.w_gpr i v) :: rest =>
+--       if i == gpr_idx then v else go gpr_idx rest
 
-/--
-Resolve any reads in each of `us` by looking them up in `es`.
--/
-def Update.resolveReads (es us : List Update) : List Update :=
-  match us with
-  | [] => []
-  | u :: rest =>
-    (Update.resolveRead es u) :: resolveReads es rest
+-- /--
+-- Resolve any reads in each of `us` by looking them up in `es`.
+-- -/
+-- def Update.resolveReads (es us : List Update) : List Update :=
+--   match us with
+--   | [] => []
+--   | u :: rest =>
+--     (Update.resolveRead es u) :: resolveReads es rest
 
 /--
 Aggregate `e` and `u`, assuming `u` follows `e`.
 -/
 def Expr.aggregate1 (e u : Expr) : Expr :=
   if e.curr_state == u.prev_state then
-    let u_resolved_writes := Update.resolveReads e.writes u.writes
+    let u_resolved_writes := Std.HashMap.union e.writes u.writes
     { prev_state := e.prev_state,
       curr_state := u.curr_state,
-      writes := go e.writes u_resolved_writes }
+      writes := u_resolved_writes }
   else
     -- We cannot aggregate two non-consecutive states, so we return the original
     -- StateUpdate here.
     -- TODO: We should probably throw an error here.
     e
- where go (es us : List Update) : List Update :=
-  match es, us with
-  | [], us => us
-  | es, [] => es
-  | es, u :: rest_us =>
-    go (Update.insertSorted es u) rest_us
+--  where go (es us : List Update) : List Update :=
+--   match es, us with
+--   | [], us => us
+--   | es, [] => es
+--   | es, u :: rest_us =>
+--     go (Update.insertSorted es u) rest_us
 
 /--
 info: { curr_state := 2,
   prev_state := 0,
-  writes := [ArmConstr.Update.w_gpr 0x00#5 (ArmConstr.GPRVal.var 1),
-             ArmConstr.Update.w_gpr 0x01#5 (ArmConstr.GPRVal.var 1),
-             ArmConstr.Update.w_gpr 0x02#5 (ArmConstr.GPRVal.var 3)] }
+  writes := Std.HashMap.ofList [(0x02#5, ArmConstr.GPRVal.r_gpr 0x01#5),
+             (0x01#5, ArmConstr.GPRVal.var 1),
+             (0x00#5, ArmConstr.GPRVal.var 1)] }
 -/
 #guard_msgs in
-open Expr Update in
+open Expr in
 #eval Expr.aggregate1
         { prev_state := 0,
           curr_state := 1,
-          writes := [w_gpr 0#5 (.var 1), w_gpr 1#5 (.var 3)] }
+          writes := .ofList [ (0#5, (.var 1)),  (1#5, (.var 3))] }
         { prev_state := 1,
           curr_state := 2,
-          writes := [w_gpr 1#5 (.var 1), w_gpr 2#5 (.r_gpr 1)] }
+          writes := .ofList [(1#5, (.var 1)), (2#5, (.r_gpr 1)) ] }
 
 /--
 Aggregate `es` onto `init`.
 Earlier updates appear first in `es`, and of course, `es` follows `init`.
 -/
 def Expr.aggregate (init : Expr) (es : Exprs) : Expr :=
-  match es with
-  | [] => init
-  | e :: rest => aggregate (aggregate1 init e) rest
+  es.foldl (init := init) (fun acc e => aggregate1 acc e)
+  -- match es with
+  -- | [] => init
+  -- | e :: rest => aggregate (aggregate1 init e) rest
 
-open Expr Update in
+open Expr in
 /--
 info: { curr_state := 2,
   prev_state := 0,
-  writes := [ArmConstr.Update.w_gpr 0x01#5 (ArmConstr.GPRVal.var 1),
-             ArmConstr.Update.w_gpr 0x02#5 (ArmConstr.GPRVal.var 2),
-             ArmConstr.Update.w_gpr 0x03#5 (ArmConstr.GPRVal.var 3)] }
+  writes := Std.HashMap.ofList [(0x03#5, ArmConstr.GPRVal.var 3),
+             (0x02#5, ArmConstr.GPRVal.var 2),
+             (0x01#5, ArmConstr.GPRVal.var 1)] }
 -/
 #guard_msgs in
 #eval Expr.aggregate
@@ -246,17 +283,16 @@ info: { curr_state := 2,
         [
           { prev_state := 0,
             curr_state := 1,
-            writes := [w_gpr 1#5 (.var 1),
-                       w_gpr 3#5 (.var 3)] },
+            writes := .ofList [(1#5, (.var 1)), (3#5, (.var 3))]
+          },
           { prev_state := 1,
             curr_state := 2,
-            writes := [w_gpr 1#5 (.var 1),
-                       w_gpr 2#5 (.var 2)] }
+            writes := .ofList [(1#5, (.var 1)), (2#5, (.var 2))] }
         ]
 
 /-- Does aggregating `updates` over `init` yield `final`? -/
 def Expr.isAggregated (init : Expr) (updates : Exprs) (final : Expr) : Bool :=
-  final == aggregate init updates
+  final.denote_eq? (aggregate init updates)
 
 theorem Expr.eq_true_of_isValid (ctx : Context) (init final : Expr) (updates : Exprs) :
   (Expr.isAggregated init updates final) →
@@ -268,7 +304,7 @@ theorem Expr.eq_true_of_isValid (ctx : Context) (init final : Expr) (updates : E
 -- Tests
 
 #time
-open Expr Update in
+open Expr in
 theorem completely_shadowed_updates
   (h_s1 : s1 = w (.GPR 0#5) x0 (w (.GPR 1#5) x1 s0))
   (h_s2 : s2 = w (.GPR 0#5) x0 (w (.GPR 1#5) x1 s1)) :
@@ -286,17 +322,18 @@ theorem completely_shadowed_updates
   -/
   s2 = w (.GPR 0#5) x0 (w (.GPR 1#5) x1 s0) := by
   have := (Expr.eq_true_of_isValid { Γs := [s0, s1, s2],
-                                     Γgpr := [x0, x1] }
+                                     Γgpr := .ofList [(0, x0), (1, x1)] }
           -- init
-          { prev_state := 0, curr_state := 0, writes := []}
+          { prev_state := 0, curr_state := 0, writes := ∅ }
           -- final
-          { prev_state := 0, curr_state := 2, writes := [w_gpr 0#5 (.var 0), w_gpr 1#5 (.var 1)] }
+          { prev_state := 0, curr_state := 2, writes := .ofList [(0#5, (.var 0)), (1#5, (.var 1))] }
           -- updates
-          [ { prev_state := 0, curr_state := 1, writes := [w_gpr 0#5 (.var 0), w_gpr 1#5 (.var 1)] },
-            { prev_state := 1, curr_state := 2, writes := [w_gpr 0#5 (.var 0), w_gpr 1#5 (.var 1)] } ]
-            (by decide))
-  simp only [Exprs.denote, List.foldl, true_and, and_imp] at this
-  exact this (Eq.refl s0) h_s1 h_s2
+          [ { prev_state := 0, curr_state := 1, writes := .ofList [(0#5, (.var 0)), (1#5, (.var 1))] },
+            { prev_state := 1, curr_state := 2, writes := .ofList [(0#5, (.var 0)), (1#5, (.var 1))] } ]
+            (by native_decide)) -- key point: to decide, we need to be able to abstract the vars to get a closed term!
+  simp at this
+  simp only [Exprs.denote, List.foldl_cons, true_and, List.foldl_nil, and_imp] at this
+  exact this -- we lose defeqs due to our use of HashMap.
   done
 
 open Expr Update in
@@ -385,7 +422,7 @@ theorem read_from_prev_update_test2 (s0 s1 s2 : ArmState)
             { prev_state := 1, curr_state := 2,
               writes := [w_gpr 1#5 (.var 2), w_gpr 3#5 (.r_gpr 5#5)] } ]
             (Eq.refl true))
-  simp only [Exprs.denote, List.foldl, true_and, and_imp] at this
+  simp? [Exprs.denote, List.foldl, and_imp] at this
   exact this (Eq.refl s0) h_s1 h_s2
   done
 
